dafny/BloodWarnings.dfy
@@ -49,7 +49,7 @@ class Blood {
 }
 
 
-class BloodTypeSum {
+class BloodTypeLevel {
   var blood_type: BloodType;
   var total: int;
   ghost var n: int;
@@ -83,8 +83,14 @@ class BloodTypeSum {
   }
 }
 
+predicate Critical(btl: BloodTypeLevel)
+requires btl != null && btl.Valid();
+reads btl
+{
+  btl.total <= 3
+}
 
-function volumeSum(s: seq<Blood>, bt: BloodType, i: int): int
+function typeVolumeSum(s: seq<Blood>, bt: BloodType, i: int): int
 requires 0 <= i <= |s|;
 requires forall j :: 0 <= j < |s| ==> s[j] != null && s[j].Valid()
 decreases s, i;
@@ -92,38 +98,46 @@ reads s;
 reads set x | x in s[..];
 {
   if |s| == 0 || i == 0 then 0
-  else if s[0].blood_type != bt then volumeSum(s[1..], bt, i - 1)
-  else s[0].volume + volumeSum(s[1..], bt, i - 1)
+  else if s[0].blood_type == bt then s[0].volume + typeVolumeSum(s[1..], bt, i - 1)
+  else typeVolumeSum(s[1..], bt, i - 1)
 }
 
 
-lemma volumeSumLemma(s: seq<Blood>, bt: BloodType, i: int)
+lemma {:induction s, bt, i} typeVolumeSumLemma(s: seq<Blood>, bt: BloodType, i: int)
 requires 0 <= i < |s|;
 requires forall j :: 0 <= j < |s| ==> s[j] != null && s[j].Valid();
 ensures forall j :: 0 <= j < |s| ==> s[j] != null && s[j].Valid();
-ensures s[i].blood_type == bt ==> (volumeSum(s, bt, i) + s[i].volume == volumeSum(s, bt, i + 1)) &&
-  s[i].blood_type != bt ==> (volumeSum(s, bt, i) == volumeSum(s, bt, i + 1));
+ensures (s[i].blood_type == bt ==> (typeVolumeSum(s, bt, i) + s[i].volume == typeVolumeSum(s, bt, i + 1))) &&
+  (s[i].blood_type != bt ==> (typeVolumeSum(s, bt, i) == typeVolumeSum(s, bt, i + 1)));
 decreases s;
 {
 
 }
 
 
-method BloodTypesTotals(s1: seq<Blood>) returns(s2: seq<BloodTypeSum>)
+method GetBloodLevels(s1: seq<Blood>) returns(s2: seq<BloodTypeLevel>)
 requires forall j :: 0 <= j < |s1| ==> s1[j] != null && s1[j].Valid();
+ensures forall j :: 0 <= j < |s1| ==> s1[j] != null && s1[j].Valid();
+ensures |s2| == 8;
+ensures s2[0] != null && s2[0].Valid() && s2[0].blood_type == AP && s2[0].total == typeVolumeSum(s1, AP, |s1|);
+ensures s2[1] != null && s2[1].Valid() && s2[1].blood_type == AN && s2[1].total == typeVolumeSum(s1, AN, |s1|);
+ensures s2[2] != null && s2[2].Valid() && s2[2].blood_type == BP && s2[2].total == typeVolumeSum(s1, BP, |s1|);
+ensures s2[3] != null && s2[3].Valid() && s2[3].blood_type == BN && s2[3].total == typeVolumeSum(s1, BN, |s1|);
+ensures s2[4] != null && s2[4].Valid() && s2[4].blood_type == ABP && s2[4].total == typeVolumeSum(s1, ABP, |s1|);
+ensures s2[5] != null && s2[5].Valid() && s2[5].blood_type == ABN && s2[5].total == typeVolumeSum(s1, ABN, |s1|);
+ensures s2[6] != null && s2[6].Valid() && s2[6].blood_type == OP && s2[6].total == typeVolumeSum(s1, OP, |s1|);
+ensures s2[7] != null && s2[7].Valid() && s2[7].blood_type == ON && s2[7].total == typeVolumeSum(s1, ON, |s1|);
+ensures forall j :: 0 <= j < |s2| ==> s2[j] != null && s2[j].Valid();
 {
-  var aps := new BloodTypeSum(AP);
-  var ans := new BloodTypeSum(AN);
-  var bps := new BloodTypeSum(BP);
-  var bns := new BloodTypeSum(BN);
-  var abps := new BloodTypeSum(ABP);
-  var abns := new BloodTypeSum(ABN);
-  var ops := new BloodTypeSum(OP);
-  var ons := new BloodTypeSum(ON);
+  var aps := new BloodTypeLevel(AP);
+  var ans := new BloodTypeLevel(AN);
+  var bps := new BloodTypeLevel(BP);
+  var bns := new BloodTypeLevel(BN);
+  var abps := new BloodTypeLevel(ABP);
+  var abns := new BloodTypeLevel(ABN);
+  var ops := new BloodTypeLevel(OP);
+  var ons := new BloodTypeLevel(ON);
   var i := 0;
-  var total := 0;
-
-  assert aps.total == 0;
 
   while i < |s1|
   invariant 0 <= i <= |s1|
@@ -134,27 +148,105 @@ requires forall j :: 0 <= j < |s1| ==> s1[j] != null && s1[j].Valid();
   invariant aps.blood_type == AP && ans.blood_type == AN && bps.blood_type == BP &&
     bns.blood_type == BN && abps.blood_type == ABP && abns.blood_type == ABN && 
     ops.blood_type == OP && ons.blood_type == ON;
-  invariant total == volumeSum(s1, AP, i);
-  decreases |s1| - i
+  invariant aps.total == typeVolumeSum(s1, AP, i) && ans.total == typeVolumeSum(s1, AN, i);
+  invariant bps.total == typeVolumeSum(s1, BP, i) && bns.total == typeVolumeSum(s1, BN, i);
+  invariant abps.total == typeVolumeSum(s1, ABP, i) && abns.total == typeVolumeSum(s1, ABN, i);
+  invariant ops.total == typeVolumeSum(s1, OP, i) && ons.total == typeVolumeSum(s1, ON, i);
+  decreases |s1| - i;
   {
     if s1[i].blood_type == AP {
       aps.AddToTotal(s1[i].volume);
-      total := total + s1[i].volume;
-      volumeSumLemma(s1, AP, i);
     } else if s1[i].blood_type == AN {
-      aps.AddToTotal(s1[i].volume);
+      ans.AddToTotal(s1[i].volume);
     } else if s1[i].blood_type == BP {
-      aps.AddToTotal(s1[i].volume);
+      bps.AddToTotal(s1[i].volume);
     } else if s1[i].blood_type == BN {
-      aps.AddToTotal(s1[i].volume);
+      bns.AddToTotal(s1[i].volume);
     } else if s1[i].blood_type == ABP {
-      aps.AddToTotal(s1[i].volume);
+      abps.AddToTotal(s1[i].volume);
     } else if s1[i].blood_type == ABN {
-      aps.AddToTotal(s1[i].volume);
+      abns.AddToTotal(s1[i].volume);
+    } else if s1[i].blood_type == OP {
+      ops.AddToTotal(s1[i].volume);
+    } else if s1[i].blood_type == ON {
+      ons.AddToTotal(s1[i].volume);
     }
+
+    typeVolumeSumLemma(s1, AP, i);
+    typeVolumeSumLemma(s1, AN, i);
+    typeVolumeSumLemma(s1, BP, i);
+    typeVolumeSumLemma(s1, BN, i);
+    typeVolumeSumLemma(s1, ABP, i);
+    typeVolumeSumLemma(s1, ABN, i);
+    typeVolumeSumLemma(s1, OP, i);
+    typeVolumeSumLemma(s1, ON, i);
 
     i := i + 1;
   }
 
   s2 := [aps, ans, bps, bns, abps, abns, ops, ons];
+}
+
+
+// This will take some time because of the number of proof obligation but it does mirror implementation
+method Main() 
+{
+  var b1 := new Blood(1, AP, 3, true, 100, "UNSW", "John Doe", "Donor01@gmail.com", false);
+  var b2 := new Blood(2, AN, 3, true, 90, "UNSW", "Steve Doe", "Donor02@gmail.com", false);
+  var b3 := new Blood(3, BN, 2, true, 70, "UNSW", "Kate Doe", "Donor03@gmail.com", false);
+  var b4 := new Blood(4, AP, 8, true, 60, "UNSW", "Kale Doe", "Donor04@gmail.com", false);
+  var b5 := new Blood(5, OP, 3, true, 30, "UNSW", "Peter Doe", "Donor05@gmail.com", false);
+  var b6 := new Blood(6, AP, 10, true, 40, "UNSW", "Parker Doe", "Donor06@gmail.com", false);
+  var b7 := new Blood(7, AN, 5, true, 40, "UNSW", "Paul Doe", "Donor07@gmail.com", false);
+
+  assert b1 != null && b1.Valid();
+  assert b2 != null && b2.Valid();
+  assert b3 != null && b3.Valid();
+  assert b4 != null && b4.Valid();
+  assert b5 != null && b5.Valid();
+  assert b6 != null && b6.Valid();
+  assert b7 != null && b7.Valid();
+
+  var s1: seq<Blood> := [b1, b2, b3, b4, b5, b6, b7];
+
+  assert s1[0] == b1 && s1[0] != null && s1[0].Valid();
+  assert s1[1] == b2 && s1[1] != null && s1[1].Valid();
+  assert s1[2] == b3 && s1[2] != null && s1[2].Valid();
+  assert s1[3] == b4 && s1[3] != null && s1[3].Valid();
+  assert s1[4] == b5 && s1[4] != null && s1[4].Valid();
+  assert s1[5] == b6 && s1[5] != null && s1[5].Valid();
+  assert s1[6] == b7 && s1[6] != null && s1[6].Valid();
+  assert forall j :: 0 <= j < |s1| ==> s1[j] != null && s1[j].Valid();
+
+  var s2 := GetBloodLevels(s1);
+  assert |s2| == 8;
+  assert s2[0] != null && s2[0].Valid() && s2[0].blood_type == AP && s2[0].total == typeVolumeSum(s1, AP, |s1|);
+  assert s2[1] != null && s2[1].Valid() && s2[1].blood_type == AN && s2[1].total == typeVolumeSum(s1, AN, |s1|);
+  assert s2[2] != null && s2[2].Valid() && s2[2].blood_type == BP && s2[2].total == typeVolumeSum(s1, BP, |s1|);
+  assert s2[3] != null && s2[3].Valid() && s2[3].blood_type == BN && s2[3].total == typeVolumeSum(s1, BN, |s1|);
+  assert s2[4] != null && s2[4].Valid() && s2[4].blood_type == ABP && s2[4].total == typeVolumeSum(s1, ABP, |s1|);
+  assert s2[5] != null && s2[5].Valid() && s2[5].blood_type == ABN && s2[5].total == typeVolumeSum(s1, ABN, |s1|);
+  assert s2[6] != null && s2[6].Valid() && s2[6].blood_type == OP && s2[6].total == typeVolumeSum(s1, OP, |s1|);
+  assert s2[7] != null && s2[7].Valid() && s2[7].blood_type == ON && s2[7].total == typeVolumeSum(s1, ON, |s1|);
+  assert forall j :: 0 <= j < |s2| ==> s2[j] != null && s2[j].Valid();
+
+  var i := 0;
+  var critical := false;
+
+  while i < |s2|
+  invariant 0 <= i <= |s2|;
+  invariant forall j :: 0 <= j < |s2| ==> s2[j] != null && s2[j].Valid();
+  decreases |s2| - i;
+  {
+    critical := false;
+
+    if s2[i].total <= 3 {
+      critical := true;
+    }
+
+    assert critical == Critical(s2[i]);
+    print s2[i].blood_type, " ", s2[i].total, " ", critical, "\n";
+     
+    i := i + 1;
+  }
 }
